src/3d/Translate.fsti
@@ -30,3 +30,6 @@ val translate_decls
   (senv:TypeSizes.size_env)
   (tenv:translate_env)
   (d:list A.decl) : ML (list T.decl & translate_env)
+
+val finish_module (en:translate_env) (mname:string) (e_and_p:list A.ident' & list A.ident')
+  : ML translate_env
